atomic_of_push.

Atomics.thy
@@ -44,6 +44,10 @@ oops
 
 subsection \<open>Derived Properties\<close>
 
+text \<open>the postcondition may be weakened (i.e. made larger, accepting more states).\<close>
+lemma wp\<^sub>\<alpha>_mono: "Q \<subseteq> Q' \<Longrightarrow> wp\<^sub>\<alpha> \<alpha> Q \<subseteq> wp\<^sub>\<alpha> \<alpha> Q'"
+unfolding wp_def by auto
+
 text \<open>Re-establish an atomic judgement over a stronger stable precondition\<close>
 lemma atomic_pre:
   assumes "R,G \<turnstile>\<^sub>A P {\<alpha>} Q" "P' \<subseteq> P" "stable R P'"
@@ -85,36 +89,43 @@ lemma atomic_falseI [intro]:
   using assms unfolding atomic_rule_def by auto
 
 
-abbreviation (input) stabilise :: "'b rel \<Rightarrow> 'b set \<Rightarrow> 'b set" where
+definition stabilise :: "'b rel \<Rightarrow> 'b set \<Rightarrow> 'b set" where
 "stabilise R P \<equiv> P \<union> R\<^sup>+ `` P"
 
-lemma "stabilise R P = (R\<^sup>*) `` P"
+lemma stabilise_rtrancl: "stabilise R P = (R\<^sup>*) `` P"
+unfolding stabilise_def
 by (simp add: Un_Image Un_commute rtrancl_trancl_reflcl)
 
 lemma stable_stabilise: "stable R (stabilise R P)"
-unfolding stable_rel
+unfolding stable_rel stabilise_def
 by auto (metis ImageI Transitive_Closure.trancl_into_trancl)
 
 lemma stabilise_supset: "P \<subseteq> stabilise R P"
+unfolding stabilise_def
 by auto
 
 lemma stabilise_stable: "stable R P \<Longrightarrow> stabilise R P = P"
-unfolding stable_rel
+unfolding stable_rel stabilise_def
 by (erule Image_closed_trancl')
 
 lemma stabilise_inter_P: "stabilise R (P1 \<inter> P2) \<subseteq> stabilise R P1 \<inter> stabilise R P2"
+unfolding stabilise_def
 by auto
 
 lemma stabilise_inter_R1: "stabilise (R1 \<inter> R2) P \<subseteq> stabilise R1 P"
+unfolding stabilise_def
 by safe (metis Int_lower1 rev_ImageI trancl_mono)
 
 lemma stabilise_inter_R2: "stabilise (R1 \<inter> R2) P \<subseteq> stabilise R2 P"
 by (metis stabilise_inter_R1 Int_commute)
 
+
 lemma stabilise_inter_RP: "stabilise (R1 \<inter> R2) (P1 \<inter> P2) \<subseteq> stabilise R1 P1 \<inter> stabilise R2 P2"
+unfolding stabilise_def
 by (safe; meson Image_iff inf_sup_ord(1,2) trancl_mono)
 
 lemma stabilise_mono_P: "P \<subseteq> P' \<Longrightarrow> stabilise R P \<subseteq> stabilise R P'"
+unfolding stabilise_def
 by auto
 
 lemma stabilise_mono_R: "R \<subseteq> R' \<Longrightarrow> stabilise R P \<subseteq> stabilise R' P"
@@ -124,7 +135,40 @@ lemma stabilise_mono_RP: "R \<subseteq> R' \<Longrightarrow> P \<subseteq> P' \<
 by (metis stabilise_mono_P stabilise_mono_R subset_trans)
 
 lemma stabilise_pushrel: "stabilise (pushrelSame R) (pushpred s P) = pushpred s (stabilise R P)"
+unfolding stabilise_def
 by (simp add: pushpred_relimage pushpred_union pushrelSame_trancl)
+
+lemma stabilise_atomic: "R,G \<turnstile>\<^sub>A P {c} Q \<Longrightarrow> R,G \<turnstile>\<^sub>A stabilise R P {c} Q"
+unfolding atomic_rule_def
+by (simp add: stabilise_stable)
+
+lemma stabilise_atomic_post: "R,G \<turnstile>\<^sub>A P {c} Q \<Longrightarrow> R,G \<turnstile>\<^sub>A P {c} stabilise R Q"
+unfolding atomic_rule_def
+by (simp add: stabilise_stable)
+
+lemma stabilise_min: "P \<subseteq> P' \<Longrightarrow> stable R P' \<Longrightarrow> stabilise R P \<subseteq> P'"
+unfolding stabilise_rtrancl
+by auto (metis stable_transitive subset_iff)
+
+
+text \<open>Manually computing the strongest postcondition which might hold.\<close>
+definition sp :: "('a,'b) basic \<Rightarrow> 'b pred \<Rightarrow> 'b pred" where
+  "sp \<alpha> P \<equiv> beh \<alpha> `` (P)"
+
+lemma wp_sp: "P \<subseteq> vc \<alpha> \<Longrightarrow> P \<subseteq> Domain (beh \<alpha>) \<Longrightarrow> P \<subseteq> wp\<^sub>\<alpha> \<alpha> (sp \<alpha> P)"
+unfolding sp_def wp_def
+by auto
+
+lemma sp_wp: "sp \<alpha> (wp\<^sub>\<alpha> \<alpha> Q) \<subseteq> Q"
+unfolding sp_def wp_def
+by auto
+
+lemma sp_mono: "P \<subseteq> P' \<Longrightarrow> sp \<alpha> P \<subseteq> sp \<alpha> P'"
+unfolding sp_def by auto
+
+lemma sp_pushbasic: "sp (pushbasic s s' \<alpha>) (pushpred s P) = pushpred s' (sp \<alpha> P)" 
+unfolding pushpred_def pushrel_def sp_def
+by auto (metis ImageI popl_push)
 
 
 text \<open>Definitions and lemmas for capturing guarantee and stability properties.\<close>
@@ -152,37 +196,37 @@ lemma guar\<^sub>\<alpha>_rel: "guar\<^sub>\<alpha> \<alpha> G = (Id_on (vc \<al
 unfolding guar_def by fast
 
 lemma guar_uncapE:
-  "guar\<^sub>\<alpha> (uncapBasic s \<alpha>) (uncapGuar G) \<Longrightarrow> guar\<^sub>\<alpha> \<alpha> G"
+  "guar\<^sub>\<alpha> (pushbasic s s' \<alpha>) (uncapGuar G) \<Longrightarrow> guar\<^sub>\<alpha> \<alpha> G"
 unfolding guar\<^sub>\<alpha>_rel
 proof -
-  assume assms: "Id_on (vc (uncapBasic s \<alpha>)) O beh (uncapBasic s \<alpha>) \<subseteq> uncapGuar G"
-  have "capGuar (Id_on (uncapPred s (vc \<alpha>)) O uncapBeh s (beh \<alpha>)) = Id_on (vc \<alpha>) O beh \<alpha>"
+  assume assms: "Id_on (vc (pushbasic s s' \<alpha>)) O beh (pushbasic s s' \<alpha>) \<subseteq> uncapGuar G"
+  have "capGuar (Id_on (uncapPred s (vc \<alpha>)) O uncapBeh s s' (beh \<alpha>)) = Id_on (vc \<alpha>) O beh \<alpha>"
     by (simp add: poprel_relcomp_pushpred)
   thus "Id_on (vc \<alpha>) O beh \<alpha> \<subseteq> G"
     using poprel_mono[OF assms] by simp
 qed
 
 lemma guar_uncapI:
-  "guar\<^sub>\<alpha> \<alpha> G \<Longrightarrow> guar\<^sub>\<alpha> (uncapBasic s \<alpha>) (uncapGuar G)"
+  "guar\<^sub>\<alpha> \<alpha> G \<Longrightarrow> guar\<^sub>\<alpha> (pushbasic s s' \<alpha>) (uncapGuar G)"
 unfolding guar\<^sub>\<alpha>_rel
 proof -
   assume "Id_on (vc \<alpha>) O beh \<alpha> \<subseteq> G"
-  hence subset: "pushrel s (Id_on (vc \<alpha>) O beh \<alpha>) \<subseteq> pushrel s G"
+  hence subset: "pushrel s s' (Id_on (vc \<alpha>) O beh \<alpha>) \<subseteq> pushrel s s' G"
     by simp
-  have "pushrel s (Id_on (vc \<alpha>) O beh \<alpha>) = Id_on (pushpred s (vc \<alpha>)) O pushrel s (beh \<alpha>)"
+  have "pushrel s s' (Id_on (vc \<alpha>) O beh \<alpha>) = Id_on (pushpred s (vc \<alpha>)) O pushrel s s' (beh \<alpha>)"
     by (rule pushrel_relcomp_id)
-  hence "Id_on (pushpred s (vc \<alpha>)) O pushrel s (beh \<alpha>) \<subseteq> pushrel s G" 
+  hence "Id_on (pushpred s (vc \<alpha>)) O pushrel s s' (beh \<alpha>) \<subseteq> pushrel s s' G" 
     using subset by simp
-  thus "Id_on (vc (uncapBasic s \<alpha>)) O beh (uncapBasic s \<alpha>) \<subseteq> uncapGuar G"
-    using pushrel_in_pushrelAll by auto
+  thus "Id_on (vc (pushbasic s s' \<alpha>)) O beh (pushbasic s s' \<alpha>) \<subseteq> uncapGuar G"
+    using pushrel_in_pushrelAll[of s s'] by auto
 qed
 
 
 lemma guar_mix:
-  "guar\<^sub>\<alpha> (capBasic \<alpha>) G \<Longrightarrow> guar\<^sub>\<alpha> \<alpha> (uncapGuar G)"
+  "guar\<^sub>\<alpha> (popbasic \<alpha>) G \<Longrightarrow> guar\<^sub>\<alpha> \<alpha> (uncapGuar G)"
 unfolding guar\<^sub>\<alpha>_rel
 proof -
-  assume "Id_on (vc (capBasic \<alpha>)) O beh (capBasic \<alpha>) \<subseteq> G"
+  assume "Id_on (vc (popbasic \<alpha>)) O beh (popbasic \<alpha>) \<subseteq> G"
   hence "Id_on (poppred (vc \<alpha>)) O poprel (beh \<alpha>) \<subseteq> G" by simp
   hence "pushrelAll (Id_on (poppred (vc \<alpha>))) O pushrelAll (poprel (beh \<alpha>)) \<subseteq> pushrelAll G"       
     by (metis pushrelAll_relcomp pushrelAll_mono)
@@ -195,10 +239,10 @@ qed
 
 
 lemma guar_capE:
-  "guar\<^sub>\<alpha> (capBasic \<alpha>) (capGuar G) \<Longrightarrow> guar\<^sub>\<alpha> \<alpha> G"
+  "guar\<^sub>\<alpha> (popbasic \<alpha>) (capGuar G) \<Longrightarrow> guar\<^sub>\<alpha> \<alpha> G"
 unfolding guar\<^sub>\<alpha>_rel
 proof -
-  assume "Id_on (vc (capBasic \<alpha>)) O beh (capBasic \<alpha>) \<subseteq> capGuar G"
+  assume "Id_on (vc (popbasic \<alpha>)) O beh (popbasic \<alpha>) \<subseteq> capGuar G"
   hence "uncapGuar (Id_on (capPred (vc \<alpha>))) O beh \<alpha> \<subseteq> G"
   sorry
   thus "Id_on (vc \<alpha>) O beh \<alpha> \<subseteq> G"
@@ -206,38 +250,65 @@ proof -
 oops
 
 lemma guar_capI:
-  "guar\<^sub>\<alpha> \<alpha> G \<Longrightarrow> guar\<^sub>\<alpha> (capBasic \<alpha>) (capGuar G)"
+  "guar\<^sub>\<alpha> \<alpha> G \<Longrightarrow> guar\<^sub>\<alpha> (popbasic \<alpha>) (capGuar G)"
 unfolding guar\<^sub>\<alpha>_rel
 proof -
   assume "Id_on (vc \<alpha>) O beh \<alpha> \<subseteq> G"
-  hence "capGuar (Id_on (vc \<alpha>)) O capGuar (beh \<alpha>) \<subseteq> capGuar G"
+  hence "poprel (Id_on (vc \<alpha>) O beh \<alpha>) \<subseteq> poprel G" by simp
+  hence "poprel (Id_on (vc \<alpha>)) O poprel (beh \<alpha>) \<subseteq> poprel G"
     using poprel_relcomp poprel_mono sorry
   moreover have "Id_on (capPred (vc \<alpha>)) = capGuar (Id_on (vc \<alpha>))"
     using poppred_eq_poprel by auto
-  ultimately show "Id_on (vc (capBasic \<alpha>)) O beh (capBasic \<alpha>) \<subseteq> capGuar G"
+  ultimately show "Id_on (vc (popbasic \<alpha>)) O beh (popbasic \<alpha>) \<subseteq> capGuar G"
     by auto
 oops
 
 
 
-lemma cap_wp_capBasic:
-  "capPred (wp\<^sub>\<alpha> (uncapBasic s \<alpha>) (uncapPred s' Q)) = wp\<^sub>\<alpha> \<alpha> Q"
+lemma cap_wp_popbasic:
+  "capPred (wp\<^sub>\<alpha> (pushbasic s s' \<alpha>) (uncapPred s' Q)) = wp\<^sub>\<alpha> \<alpha> Q"
 proof -
   have
-    "capPred {m. \<forall>m'. (m, m') \<in> beh (uncapBasic s \<alpha>) \<longrightarrow> m' \<in> uncapPred s' Q}
+    "capPred {m. \<forall>m'. (m, m') \<in> beh (pushbasic s s' \<alpha>) \<longrightarrow> m' \<in> uncapPred s' Q}
       = {m. \<forall>m'. (m, m') \<in> beh \<alpha> \<longrightarrow> m' \<in> Q}"
       unfolding pushpred_def pushrel_def poppred_def
       apply auto sorry
-  moreover have "capPred (vc (uncapBasic s \<alpha>)) = vc \<alpha>" by force
-  moreover have "capPred (Domain (beh (uncapBasic s \<alpha>))) = Domain (beh \<alpha>)"
+  moreover have "capPred (vc (pushbasic s s' \<alpha>)) = vc \<alpha>" by force
+  moreover have "capPred (Domain (beh (pushbasic s s' \<alpha>))) = Domain (beh \<alpha>)"
     unfolding poppred_def pushrel_def poprel_def by force
   ultimately show ?thesis using wp_rel_partial poppred_inter
 oops
 
+lemma atomic_push:
+  assumes "pushrelSame R,pushrelAll G \<turnstile>\<^sub>A pushpred s P {pushbasic s s' \<alpha>} pushpred s' Q"
+  shows "R,G \<turnstile>\<^sub>A P {\<alpha>} Q"
+using assms
+unfolding atomic_rule_def
+proof (intro conjI)
+  assume "pushpred s P \<subseteq> wp\<^sub>\<alpha> (tag \<alpha>, pushpred s (vc \<alpha>), pushrel s s' (beh \<alpha>)) (pushpred s' Q) \<and>
+    guar\<^sub>\<alpha> (tag \<alpha>, pushpred s (vc \<alpha>), pushrel s s' (beh \<alpha>)) (pushrelAll G) \<and>
+    stable (pushrelSame R) (pushpred s P) \<and> stable (pushrelSame R) (pushpred s' Q)"
+  hence prems:
+    "pushpred s P \<subseteq> wp\<^sub>\<alpha> (pushbasic s s' \<alpha>) (pushpred s' Q)"
+    "guar\<^sub>\<alpha> (pushbasic s s' \<alpha>) (pushrelAll G)"
+    "stable (pushrelSame R) (pushpred s P)"
+    "stable (pushrelSame R) (pushpred s' Q)"
+    by auto
+  thus "stable R P" "stable R Q"
+    using stable_uncap by auto
+  have "poppred (pushpred s P) \<subseteq> wp\<^sub>\<alpha> \<alpha> Q" 
+    (* using cap_wp_popbasic poppred_mono by blast *)
+    sorry
+  thus "P \<subseteq> wp\<^sub>\<alpha> \<alpha> Q" by simp
+  show "guar\<^sub>\<alpha> \<alpha> G" using prems(2) (* guar_capI *) sorry
+oops
+  
 
-lemma atomic_uncap:
+
+
+(* lemma atomic_uncap:
   assumes "uncapRely R,uncapGuar G \<turnstile>\<^sub>A 
-    uncapPred s P {uncapBasic s \<alpha>} uncapPred s' Q"
+    uncapPred s P {pushbasic s \<alpha>} uncapPred s' Q"
     (is "?ucR,?ucG \<turnstile>\<^sub>A ?ucP {?uca} ?ucQ")
   shows "R,G \<turnstile>\<^sub>A P {\<alpha>} Q"
 unfolding atomic_rule_def
@@ -250,11 +321,11 @@ proof (intro conjI)
     using stable_uncap by auto
   have "capPred ?ucP \<subseteq> wp\<^sub>\<alpha> \<alpha> Q" 
     using assms'(1)
-    (* using cap_wp_capBasic poppred_mono by blast *)
+    (* using cap_wp_popbasic poppred_mono by blast *)
     sorry
   thus "P \<subseteq> wp\<^sub>\<alpha> \<alpha> Q" by simp
   show "guar\<^sub>\<alpha> \<alpha> G" using assms'(2)
     by (simp add: guar_uncapE)
-oops
+oops *)
 
 end
