Semantics.thy
@@ -33,15 +33,12 @@ inductive lexecute :: "('a,'b) com \<Rightarrow> ('a,'b) com \<Rightarrow> ('a,'
   ino[intro]: "c\<^sub>1 \<mapsto>[r,\<alpha>] c\<^sub>1' \<Longrightarrow> c\<^sub>1 ;; c\<^sub>2 \<mapsto>[r,\<alpha>] c\<^sub>1' ;; c\<^sub>2" |
   ord[intro]: "c\<^sub>1 \<mapsto>[r,\<alpha>] c\<^sub>1' \<Longrightarrow> c\<^sub>1 \<cdot> c\<^sub>2 \<mapsto>[r,\<alpha>] c\<^sub>1' \<cdot> c\<^sub>2" |
   ooo[intro]: "c\<^sub>1 \<mapsto>[r,\<alpha>] c\<^sub>1' \<Longrightarrow> \<alpha>' < c\<^sub>2 ;; r <\<^sub>c \<alpha> \<Longrightarrow> c\<^sub>2 ;; c\<^sub>1 \<mapsto>[c\<^sub>2 ;; r ,\<alpha>] c\<^sub>2 ;; c\<^sub>1'"
-  | cap[intro]: "c \<mapsto>[uncapCom s r,uncapBasic s \<alpha>] c' 
-    \<Longrightarrow> Capture s c \<mapsto>[r,\<alpha>] Capture s c'"
+  | cap[intro]: "c \<mapsto>[Capture s r,pushbasic s s' \<alpha>] c' \<Longrightarrow> Capture s c \<mapsto>[r,\<alpha>] Capture s' c'"
 (*   cap[intro]: "c\<^sub>1 \<mapsto>[r,\<alpha>] c\<^sub>1' \<Longrightarrow> 
     Capture s c\<^sub>1 \<mapsto>[Nil,
       (tag \<alpha>\<llangle>r\<rrangle>, {m. merge m s \<in> vc \<alpha>\<llangle>r\<rrangle>}, {(m,m'). (merge m s, merge m' s') \<in> beh \<alpha>\<llangle>r\<rrangle>})] 
     Capture s' c\<^sub>1'" *)
-  (* | capNil[intro]: "c\<^sub>1 \<mapsto>[r,\<alpha>] c\<^sub>1' \<Longrightarrow> Capture s c\<^sub>1 \<mapsto>[f r,capBasi
-
-c \<alpha>\<llangle>r\<rrangle> s s'] Capture s' c\<^sub>1'"  *)
+  (* | capNil[intro]: "c\<^sub>1 \<mapsto>[r,\<alpha>] c\<^sub>1' \<Longrightarrow> Capture s c\<^sub>1 \<mapsto>[f r,capBasic \<alpha>\<llangle>r\<rrangle> s s'] Capture s' c\<^sub>1'"  *)
 inductive_cases lexecuteE[elim]: "c \<mapsto>[p,\<alpha>] c'"
 
 inductive gexecute :: "('a,'b) com \<Rightarrow> 'b rel \<Rightarrow> ('a,'b) com \<Rightarrow> bool"
@@ -149,7 +146,7 @@ lemma [simp]:
   by (induct s) auto
 
 lemma basics_exec:
-  assumes "lexecute c r \<alpha> c'" shows "basics c \<supseteq> basics c'"
+  assumes "c \<mapsto>[r,\<alpha>] c'" shows "basics c \<supseteq> basics c'"
   using assms by induct auto
 
 lemma basics_silent:
@@ -157,8 +154,17 @@ lemma basics_silent:
   using assms basics_exec by (induct) auto   
 
 
-lemma seqonly_uncapCom [simp]: "seqonly (uncapCom s c) = seqonly c"
-by induct auto
+fun seqonly :: "('a,'b) com \<Rightarrow> bool" where
+  "seqonly Nil = True" |
+  "seqonly (Basic _) = True" |
+  "seqonly (Seq c1 c2) = (seqonly c1 \<and> seqonly c2)" |
+  "seqonly (Ord c1 c2) = (seqonly c1 \<and> seqonly c2)" |
+  "seqonly _ = False"
+
+
+
+(* lemma seqonly_popcom [simp]: "seqonly (popcom c) = seqonly c"
+by induct auto *)
 
 lemma seqonly_reorder_com [simp]: "\<alpha>' < c <\<^sub>c \<alpha> \<Longrightarrow> seqonly c"
 by (induct rule: reorder_com.induct) auto
@@ -166,31 +172,86 @@ by (induct rule: reorder_com.induct) auto
 lemma seqonly_lexecute [simp]: "c \<mapsto>[r,\<alpha>] c' \<Longrightarrow> seqonly r"
 by (induct rule: lexecute.induct) auto
 
-lemma capBasic_uncapCom:
+(* lemma popbasic_pushcom:
   assumes "seqonly r"
-  shows "capBasic ` basics (uncapCom s r) = basics r"
+  shows "popbasic ` basics (pushcom s r) = basics r"
 using assms
 proof (induct r)
   case (Basic \<alpha>)
-  have "capBasic ` {uncapBasic s \<alpha>} = {\<alpha>}"
-    by simp
+  have "popbasic ` {pushbasic s \<alpha>} = {\<alpha>}" by simp
   thus ?case by simp
-qed (auto simp add: image_Un)
+qed (auto simp add: image_Un) *)
 
-lemma basics_exec_prefix:
-  assumes "lexecute c r \<alpha> c'" shows "basics c \<supseteq> insert \<alpha> (basics r)"
+(* lemma basics_exec_prefix:
+  assumes "c \<mapsto>[r,\<alpha>] c'" shows "basics c \<supseteq> insert \<alpha> (basics r)"
   using assms
 proof (induct rule: lexecute.induct)
-  case (cap c s r \<alpha> c')
+  case (cap c s r \<alpha> c' s')
   hence "seqonly r" using seqonly_lexecute by fastforce
-  hence "capBasic ` basics (uncapCom s r) = basics r"
-    by (rule capBasic_uncapCom)
-  hence "basics r \<subseteq> capBasic ` basics c"
+  hence "popbasic ` basics (pushcom s r) = basics r"
+    by (rule popbasic_pushcom)
+  hence "basics r \<subseteq> popbasic ` basics c"
     using cap(2) image_mono by fastforce
-  moreover have "\<alpha> \<in> capBasic ` basics c"
+  moreover have "\<alpha> \<in> popbasic ` basics c"
     using cap(2) image_iff by fastforce
   ultimately show ?case by simp
-qed auto
+qed auto *)
+
+text \<open>If P satisfies the wp of a pushbasic, then it must have had 's' pushed onto it.\<close>
+lemma wp_of_push_poppable:
+  assumes "P \<subseteq> wp\<^sub>\<alpha> (pushbasic s s' \<alpha>) Q"
+  shows "P = pushpred s (poppred P)" 
+using assms
+unfolding wp_rel
+proof -
+  have dom: "Domain (beh (pushbasic s s' \<alpha>)) = pushpred s (Domain (beh \<alpha>))"
+    unfolding pushpred_def pushrel_def by auto
+  assume assms': "P \<subseteq> vc (pushbasic s s' \<alpha>) \<inter> Domain (beh (pushbasic s s' \<alpha>)) \<inter> - (beh (pushbasic s s' \<alpha>))\<inverse> `` (- Q)"
+  hence "P \<subseteq> pushpred s (Domain (beh \<alpha>))" using dom by simp
+  thus ?thesis by (rule pushpred_poppred_id)
+qed
+
+lemma atomic_of_push:
+  assumes "pushrelSame R,G \<turnstile>\<^sub>A P {pushbasic s s' \<alpha>} Q"
+  shows "\<exists>Q'. Q' \<subseteq> Q \<and> Q' = pushpred s' (poppred Q') \<and> pushrelSame R,G \<turnstile>\<^sub>A P {pushbasic s s' \<alpha>} Q'"
+unfolding atomic_rule_def
+proof (intro exI conjI)
+  have assms':
+    "P \<subseteq> wp\<^sub>\<alpha> (pushbasic s s' \<alpha>) Q"
+
+    "P \<subseteq> vc (pushbasic s s' \<alpha>)"
+    "P \<subseteq> Domain (beh (pushbasic s s' \<alpha>))"
+    "P \<subseteq> - (beh (pushbasic s s' \<alpha>))\<inverse> `` (- Q)"
+
+    "guar\<^sub>\<alpha> (pushbasic s s' \<alpha>) G"
+    "stable (pushrelSame R) P"
+    "stable (pushrelSame R) Q"
+    using assms unfolding atomic_rule_def wp_rel by auto
+  thus "stable (pushrelSame R) P" "guar\<^sub>\<alpha> (pushbasic s s' \<alpha>) G" by simp+
+
+  let ?Q' = "stabilise (pushrelSame R) (sp (pushbasic s s' \<alpha>) P)"
+  show "stable (pushrelSame R) ?Q'" by (rule stable_stabilise)
+
+  have "P = pushpred s (poppred P)" using assms' by (simp add: wp_of_push_poppable)
+  hence "sp (pushbasic s s' \<alpha>) P = sp (pushbasic s s' \<alpha>) (pushpred s (poppred P))" by simp
+  also have "... = pushpred s' (sp \<alpha> (poppred P))" 
+    using sp_pushbasic by fast
+  finally have sp: "sp (pushbasic s s' \<alpha>) P = pushpred s' (sp \<alpha> (poppred P))" by simp
+
+  hence "sp (pushbasic s s' \<alpha>) P = pushpred s' (poppred (sp (pushbasic s s' \<alpha>) P))"
+    using pushpred_poppred_id by simp
+  hence "?Q' = pushpred s' (stabilise R (sp \<alpha> (poppred P)))"
+    using stabilise_pushrel sp by metis
+  thus "?Q' = pushpred s' (poppred ?Q')" by simp
+
+  have "P \<subseteq> wp\<^sub>\<alpha> (pushbasic s s' \<alpha>) (sp (pushbasic s s' \<alpha>) P)"
+    using assms'(2,3) by (intro wp_sp, auto)
+  thus "P \<subseteq> wp\<^sub>\<alpha> (pushbasic s s' \<alpha>) ?Q'"
+    using stabilise_supset[of "sp (pushbasic s s' \<alpha>) P"] wp\<^sub>\<alpha>_mono by fast
+
+  have "sp (pushbasic s s' \<alpha>) P \<subseteq> Q" using assms'(1) sp_mono sp_wp by fast
+  thus "?Q' \<subseteq> Q" using assms'(7) stabilise_min[of _ Q] by simp
+qed
 
 end
 
